Finish Act and Message cases

compiler/backend/proofs/env_to_stateProofScript.sml
@@ -32,23 +32,15 @@ Inductive compile_rel:
   (compile_rel te se ⇒
   compile_rel (Prim (Cons "Ret") [Delay te]) (Lam NONE (Delay se))) ∧
 
+[~Raise:]
+  (compile_rel te se ⇒
+  compile_rel (Prim (Cons "Raise") [Delay te]) (Lam NONE (Raise (Delay se)))) ∧
+
 [~Bind:]
   (compile_rel te1 se1 ∧ compile_rel te2 se2 ⇒
   compile_rel
-    (Prim (Cons "Bind") [te1; te2])
-    (Lam NONE $ app (app (Force se2) (app (Force se1) Unit)) Unit)) ∧
-
-[~Raise:]
-  (compile_rel te se ∧
-   u ∉ freevars se ⇒
-  compile_rel (Prim (Cons "Raise") [Delay te]) (Lam NONE $ Raise se)) ∧
-
-[~Handle:]
-  (compile_rel te1 se1 ∧ compile_rel te2 se2 ∧
-   u ∉ freevars se1 ∪ freevars se2 ∧ x ∉ freevars se2 ∧ u ≠ x ⇒
-  compile_rel
-    (Prim (Cons "Handle") [Delay te1; Delay te2])
-    (Lam (SOME u) $ Handle (app se1 (Var u)) x (app (app se2 (Var x)) (Var u)))) ∧
+    (Prim (Cons "Bind") [Delay te1; Delay te2])
+    (Lam NONE $ app (app se2 (app se1 Unit)) Unit)) ∧
 
 (*
 [~Alloc:]
@@ -71,18 +63,17 @@ Inductive compile_rel:
    EVERY (λse. u ∉ freevars se) ses ⇒
   compile_rel (Prim (Cons "Update") (MAP Delay tes)) (Lam NONE $ App Update ses)) ∧
 
-[~Act:]
-  (compile_rel te se ∧
-   u ∉ freevars se ⇒
-  compile_rel (Prim (Cons "Act") [Delay te]) (Lam (SOME u) $ app se (Var u))) ∧
+*)
 
 [~Message:]
-  (compile_rel te se ∧ u ≠ x ⇒
+  (compile_rel te se ⇒
   compile_rel
     (Prim (AtomOp (Message s)) [te])
-    (Let (SOME x) se $ Lam u $ App (FFI s) [Var x])) ∧
+    (Let (SOME x) se $ Lam NONE $ App (FFI s) [Var x])) ∧
 
-*)
+[~Act:]
+  (compile_rel te se ⇒
+  compile_rel (Prim (Cons "Act") [Delay te]) (Lam NONE (app (app se Unit) Unit))) ∧
 
 [~AtomOp:]
   (LIST_REL compile_rel tes ses ∧
@@ -135,7 +126,13 @@ Inductive compile_rel:
 [~Force:]
   (∀te se.
     compile_rel te se ⇒
-    compile_rel (Force te) (Force se))
+    compile_rel (Force te) (Force se)) (*∧
+
+[~Message:]
+  (∀te se.
+    compile_rel te se ⇒
+    compile_rel (Prim (AtomOp (Message ch)) [te])
+                (Let (SOME a) se (Lam NONE (App (FFI ch) [Var a]))))*)
 
 End
 
@@ -171,13 +168,38 @@ Inductive v_rel:
 
 [~Atom:]
   (∀a.
+     (∀msg x. ~(a = Msg msg x)) ⇒
      v_rel (Atom a) (Atom a)) ∧
+
+[~Msg:]
+  (∀msg s x senv.
+     v_rel (Atom (Msg msg s))
+           (Closure NONE ((x,Atom (Str s))::senv) (App (FFI msg) [Var x]))) ∧
+
+[~Act:]
+  (∀te se tenv senv.
+     compile_rel te se ∧ env_rel tenv senv ⇒
+     v_rel (Constructor "Act" [Thunk (INR (tenv,te))])
+           (Closure NONE senv (app (app se Unit) Unit))) ∧
 
 [~Ret:]
   (∀te se tenv senv.
      compile_rel te se ∧ env_rel tenv senv ⇒
      v_rel (Constructor "Ret" [Thunk (INR (tenv,te))])
            (Closure NONE senv (Delay se))) ∧
+
+[~Bind:]
+  (∀te1 se1 te2 se2 tenv senv.
+     compile_rel te1 se1 ∧ compile_rel te2 se2 ∧ env_rel tenv senv ⇒
+     v_rel
+       (Constructor "Bind" [Thunk (INR (tenv,te1)); Thunk (INR (tenv,te2))])
+       (Closure NONE senv (app (app se2 (app se1 Unit)) Unit))) ∧
+
+[~Raise:]
+  (∀te se tenv senv.
+     compile_rel te se ∧ env_rel tenv senv ⇒
+     v_rel (Constructor "Raise" [Thunk (INR (tenv,te))])
+           (Closure NONE senv (Raise (Delay se)))) ∧
 
 [env_rel:]
   (∀tenv senv.
@@ -262,6 +284,10 @@ Theorem v_rel_bool:
 Proof
   once_rewrite_tac [v_rel_cases] \\ fs [] \\ EVAL_TAC
 QED
+
+val step =
+  LIST_CONJ [step_def,push_def,return_def,value_def,opt_bind_def,continue_def,
+             application_def,dest_anyClosure_def,dest_Closure_def];
 
 Theorem eval_to_thm:
   ∀n tenv te tres se senv st k.
@@ -523,15 +549,89 @@ Proof
   \\ Cases_on ‘op’ \\ gvs []
   \\ TRY (fs [eval_to_def] \\ NO_TAC)
   >~ [‘Cons s’] >-
-   (Cases_on ‘s = "Ret"’ \\ gvs []
-    >-
+   (Cases_on ‘s = "Ret"’ \\ gvs [] >-
+     (simp [Once compile_rel_cases] \\ fs [monad_cns_def] \\ rw []
+      \\ fs [eval_to_def,result_map_def]
+      \\ qexists_tac ‘1’
+      \\ fs [step_def,push_def,return_def,continue_def,value_def]
+      \\ simp [Once v_rel_cases])
+    \\ Cases_on ‘s = "Act"’ \\ gvs [] >-
+     (simp [Once compile_rel_cases] \\ fs [monad_cns_def] \\ rw []
+      \\ fs [eval_to_def,result_map_def]
+      \\ simp [Once v_rel_cases,PULL_EXISTS,monad_cns_def]
+      \\ rpt (first_x_assum $ irule_at Any)
+      \\ Q.REFINE_EXISTS_TAC ‘ck1+1’ \\ rewrite_tac [step_n_add] \\ fs [step]
+      \\ qexists_tac ‘0’ \\ fs [])
+    \\ Cases_on ‘s = "Bind"’ \\ gvs [] >-
+     (simp [Once compile_rel_cases] \\ fs [monad_cns_def] \\ rw []
+      \\ fs [eval_to_def,result_map_def]
+      \\ qexists_tac ‘1’
+      \\ fs [step_def,push_def,return_def,continue_def,value_def]
+      \\ simp [Once v_rel_cases])
+    \\ Cases_on ‘s = "Raise"’ \\ gvs [] >-
      (simp [Once compile_rel_cases] \\ fs [monad_cns_def] \\ rw []
       \\ fs [eval_to_def,result_map_def]
       \\ qexists_tac ‘1’
       \\ fs [step_def,push_def,return_def,continue_def,value_def]
       \\ simp [Once v_rel_cases])
     \\ cheat)
+  >~ [‘Proj s i’] >- cheat
+  >~ [‘IsEq s i’] >- cheat
+  \\ rename [‘AtomOp a’]
+  \\ Cases_on ‘∃msg. a = Message msg’
+  >-
+   (simp [Once compile_rel_cases] \\ gvs [GSYM PULL_FORALL]
+    \\ rpt strip_tac \\ gvs []
+    \\ gvs [eval_to_def]
+    \\ Cases_on ‘n=0’ \\ gvs [result_map_def]
+    >- (qexists_tac ‘0’ \\ fs [result_map_def,is_halt_def])
+    \\ Cases_on ‘eval_to (n − 1) tenv te’ \\ fs []
+    >-
+     (Cases_on ‘x'’ \\ fs []
+      \\ first_x_assum drule_all \\ rw []
+      \\ Q.REFINE_EXISTS_TAC ‘ck1+1’ \\ rewrite_tac [step_n_add] \\ fs [step])
+    \\ gvs []
+    \\ Cases_on ‘y’ \\ gvs []
+    \\ Cases_on ‘l’ \\ gvs [eval_op_def]
+    \\ Q.REFINE_EXISTS_TAC ‘ck1+1’ \\ rewrite_tac [step_n_add] \\ fs [step]
+    \\ first_x_assum drule_all
+    \\ disch_then (qspecl_then [‘st’,
+           ‘LetK senv (SOME x) (Lam NONE (App (FFI msg) [Var x]))::k’] strip_assume_tac)
+    \\ Q.REFINE_EXISTS_TAC ‘ck1+ck’ \\ rewrite_tac [step_n_add] \\ fs [step]
+    \\ Q.REFINE_EXISTS_TAC ‘ck1+1’ \\ rewrite_tac [step_n_add] \\ fs [step]
+    \\ Q.REFINE_EXISTS_TAC ‘ck1+1’ \\ rewrite_tac [step_n_add] \\ fs [step]
+    \\ qexists_tac ‘0’ \\ fs []
+    \\ pop_assum mp_tac
+    \\ simp [Once v_rel_cases] \\ rw []
+    \\ simp [Once v_rel_cases] \\ rw [])
   \\ cheat
+QED
+
+Theorem eval_thm:
+  ∀tenv senv te se st k.
+    compile_rel te se ∧ env_rel tenv senv ⇒
+    eval tenv te = INL Type_error ∨
+    (eval tenv te = INL Diverge ∧
+     ∀n. ∃ck x1 x2 x3.
+           n ≤ ck ∧ ~is_halt (x1,x2,x3) ∧
+           step_n ck (Exp senv se, st, k) = (x1,x2,x3)) ∨
+    ∃ck tv sv.
+      eval tenv te = INR tv ∧
+      step_n ck (Exp senv se, st, k) = (Val sv,st,k) ∧ v_rel tv sv
+Proof
+  rw [] \\ Cases_on ‘eval tenv te’ \\ gvs []
+  >-
+   (Cases_on ‘x’ \\ fs [] \\ rw []
+    \\ gvs [eval_eq_Diverge]
+    \\ pop_assum $ qspec_then ‘n’ assume_tac
+    \\ drule eval_to_thm \\ fs []
+    \\ rw [] \\ pop_assum drule_all
+    \\ disch_then $ qspecl_then [‘st’,‘k’] strip_assume_tac
+    \\ ‘∃tt. step_n ck (Exp senv se,st,k) = tt’ by fs [] \\ PairCases_on ‘tt’ \\ fs []
+    \\ qexists_tac ‘ck’ \\ fs [])
+  \\ drule eval_neq_Diverge \\ gvs []
+  \\ strip_tac \\ fs []
+  \\ drule eval_to_thm \\ fs []
 QED
 
 
@@ -620,11 +720,203 @@ Proof
 QED
 
 Inductive cont_rel:
-  (∀tk. tk = env_semantics$Done ⇒
-    cont_rel tk [])
+  (cont_rel Done []) ∧
+  (∀tk sk senv tenv te se.
+    cont_rel tk sk ∧ env_rel tenv senv ∧ compile_rel te se ⇒
+    cont_rel (BC (Thunk (INR (tenv,te))) tk)
+      (AppK senv AppOp [] [se]:: AppK senv AppOp [Constructor "" []] []::sk))
 End
 
+Theorem eval_Delay:
+  eval env (Delay e) = INR (Thunk (INR (env,e)))
+Proof
+  fs [eval_def,eval_to_def]
+  \\ DEEP_INTRO_TAC some_intro \\ fs [] \\ rw []
+QED
+
+Theorem force_Thunk[simp]:
+  force (Thunk (INR (env,e))) = eval env e
+Proof
+  fs [force_def,envLangTheory.dest_anyThunk_def,dest_Thunk_def]
+QED
+
 Theorem next_thm:
+  ∀k tv sv tk sk senv tres ts ss.
+    v_rel tv sv ∧
+    LIST_REL (LIST_REL v_rel) ts ss ∧
+    cont_rel tk sk ∧
+    next k (INR tv) tk ts = tres ∧ tres ≠ Err ⇒
+    ∃n sres ss0 ss1 sk1.
+      step_n n (Val sv,SOME ss,AppK senv AppOp [Constructor "" []] []::sk) =
+          (sres,ss0,sk1) ∧
+      (tres = Div ⇒ k ≤ n ∧ ~is_halt (sres,ss0,sk1)) ∧
+      (tres = Ret ⇒ ss0 = SOME ss1 ∧
+                    is_halt (sres,ss0,sk1) ∧ ∀ch c. sres ≠ Action ch c ∧ sres ≠ Error) ∧
+      (∀a b tk ts1.
+         tres = Act (a,b) tk ts1 ⇒
+         ∃sk nenv.
+           ss0 = SOME ss1 ∧
+           sres = Action a b ∧
+           cont_rel tk sk ∧ sk1 = AppK nenv AppOp [Constructor "" []] []::sk ∧
+           LIST_REL (LIST_REL v_rel) ts1 ss1)
+Proof
+
+  gen_tac \\ completeInduct_on ‘k’
+  \\ gvs [PULL_FORALL,AND_IMP_INTRO] \\ rw []
+  \\ reverse (Cases_on ‘∃s vs. tv = Constructor s vs’)
+  >- (Cases_on ‘tv’ \\ fs [Once next_def])
+  \\ gvs []
+  \\ pop_assum mp_tac
+  \\ qpat_x_assum ‘v_rel _ _’ mp_tac
+  \\ Cases_on ‘s = "Ret"’ >-
+   (reverse (Cases_on ‘LENGTH vs = 1’) >- fs [Once next_def]
+    \\ once_rewrite_tac [next_def] \\ gvs []
+    \\ simp [Once v_rel_cases,monad_cns_def]
+    \\ strip_tac \\ gvs []
+    \\ Cases_on ‘tk’ \\ fs []
+    >-
+     (Q.REFINE_EXISTS_TAC ‘ck1+1’
+      \\ rewrite_tac [step_n_add]
+      \\ fs [step_def,push_def,return_def,value_def,opt_bind_def,continue_def,
+             application_def,dest_anyClosure_def,dest_Closure_def]
+      \\ qexists_tac ‘1’ \\ fs [step_def,value_def,GSYM PULL_FORALL]
+      \\ fs [Once cont_rel_cases,is_halt_def])
+    >-
+     (IF_CASES_TAC \\ gvs []
+      >- (qexists_tac ‘0’ \\ fs [is_halt_def])
+      \\ strip_tac
+      \\ Q.REFINE_EXISTS_TAC ‘ck1+1’ \\ rewrite_tac [step_n_add] \\ fs [step]
+      \\ Q.REFINE_EXISTS_TAC ‘ck1+1’ \\ rewrite_tac [step_n_add] \\ fs [step]
+      \\ fs [force_apply_closure_def]
+      \\ qpat_x_assum ‘cont_rel _ _’ mp_tac
+      \\ simp [Once cont_rel_cases]
+      \\ strip_tac \\ gvs []
+      \\ Q.REFINE_EXISTS_TAC ‘ck1+1’ \\ rewrite_tac [step_n_add] \\ fs [step]
+      \\ rename [‘env_rel tenv1 senv1’]
+      \\ rename [‘compile_rel te1 se1’]
+      \\ rename [‘cont_rel tk1 sk1’]
+      \\ Cases_on ‘eval tenv1 te1’
+      >-
+       (Cases_on ‘x’ \\ gvs []
+        \\ fs [eval_eq_Diverge]
+        \\ pop_assum (qspec_then ‘k’ assume_tac)
+        \\ drule eval_to_thm
+        \\ disch_then drule
+        \\ disch_then drule \\ fs []
+        \\ rename [‘(Exp senv1 se1,SOME ss,kk)’]
+        \\ disch_then (qspecl_then [‘SOME ss’,‘kk’] strip_assume_tac)
+        \\ ‘∃l. step_n ck (Exp senv1 se1,SOME ss,kk) = l’ by fs [] \\ PairCases_on ‘l’ \\ fs []
+        \\ first_x_assum $ irule_at $ Pos hd \\ fs [])
+      \\ fs []
+      \\ drule eval_neq_Diverge \\ fs [] \\ strip_tac
+      \\ rename [‘eval_to ck’]
+      \\ drule eval_to_thm
+      \\ disch_then drule
+      \\ disch_then drule \\ fs []
+      \\ qmatch_goalsub_abbrev_tac ‘step_n _ (_,SOME _,k1)’
+      \\ disch_then (qspecl_then [‘SOME ss’,‘k1’] strip_assume_tac)
+      \\ Q.REFINE_EXISTS_TAC ‘ck1+ck'’ \\ rewrite_tac [step_n_add] \\ fs [step]
+      \\ simp [Abbr‘k1’]
+      \\ Q.REFINE_EXISTS_TAC ‘ck1+1’ \\ rewrite_tac [step_n_add]
+      \\ fs [step_def,return_def]
+      \\ cheat)
+    \\ cheat)
+  \\ Cases_on ‘s = "Raise"’ >-
+   (reverse (Cases_on ‘LENGTH vs = 1’) >- fs [Once next_def]
+    \\ once_rewrite_tac [next_def] \\ fs []
+    \\ cheat)
+  \\ Cases_on ‘s = "Bind"’ >-
+   (reverse (Cases_on ‘LENGTH vs = 2’) >- fs [Once next_def]
+    \\ once_rewrite_tac [next_def] \\ fs []
+    \\ simp [Once v_rel_cases,monad_cns_def]
+    \\ strip_tac \\ gvs []
+    \\ IF_CASES_TAC \\ fs []
+    >- (qexists_tac ‘0’ \\ fs [is_halt_def])
+    \\ strip_tac
+    \\ ntac 8 (Q.REFINE_EXISTS_TAC ‘ck1+1’ \\ rewrite_tac [step_n_add] \\ fs [step])
+    \\ rename [‘step_n _ (Exp senv se1,SOME ss,_)’]
+    \\ Cases_on ‘eval tenv te1’
+    >-
+     (Cases_on ‘x’ >- fs [Once next_def]
+      \\ ntac 2 (pop_assum mp_tac) \\ once_rewrite_tac [next_def] \\ simp []
+      \\ fs [eval_eq_Diverge]
+      \\ disch_then (qspec_then ‘k’ assume_tac)
+      \\ drule eval_to_thm
+      \\ disch_then drule
+      \\ disch_then drule \\ fs []
+      \\ rename [‘(Exp senv se1,SOME ss,kk)’]
+      \\ disch_then (qspecl_then [‘SOME ss’,‘kk’] strip_assume_tac)
+      \\ ‘∃l. step_n ck (Exp senv se1,SOME ss,kk) = l’ by fs [] \\ PairCases_on ‘l’ \\ fs []
+      \\ first_x_assum $ irule_at $ Pos hd \\ fs [])
+    \\ drule eval_neq_Diverge \\ fs [] \\ strip_tac
+    \\ rename [‘eval_to ck’]
+    \\ drule eval_to_thm
+    \\ disch_then drule
+    \\ disch_then drule \\ fs []
+    \\ qmatch_goalsub_abbrev_tac ‘step_n _ (_,SOME _,k1)’
+    \\ disch_then (qspecl_then [‘SOME ss’,‘k1’] strip_assume_tac)
+    \\ Q.REFINE_EXISTS_TAC ‘ck1+ck'’ \\ rewrite_tac [step_n_add] \\ fs [step]
+    \\ last_x_assum $ drule_at $ Pos last \\ simp []
+    \\ rpt (disch_then drule)
+    \\ disch_then (qspecl_then [‘AppK senv AppOp [] [se2]::
+             AppK senv AppOp [Constructor "" []] []::sk’,‘senv’] mp_tac)
+    \\ impl_tac >- (simp [Once cont_rel_cases] \\ fs [])
+    \\ fs [] \\ strip_tac
+    \\ gvs [GSYM PULL_FORALL]
+    \\ first_x_assum $ irule_at $ Pos hd
+    \\ Cases_on ‘next (k − 1) (INR y) (BC (Thunk (INR (tenv,te2))) tk) ts’ \\ fs []
+    \\ PairCases_on ‘e’ \\ fs [])
+  \\ Cases_on ‘s = "Handle"’ >-
+   (reverse (Cases_on ‘LENGTH vs = 2’) >- fs [Once next_def]
+    \\ once_rewrite_tac [next_def] \\ fs []
+    \\ cheat)
+  \\ Cases_on ‘s = "Act"’ >-
+   (reverse (Cases_on ‘LENGTH vs = 1’) >- fs [Once next_def]
+    \\ once_rewrite_tac [next_def] \\ fs []
+    \\ simp [Once v_rel_cases,monad_cns_def] \\ rw []
+    \\ ntac 7 (Q.REFINE_EXISTS_TAC ‘ck1+1’ \\ rewrite_tac [step_n_add] \\ fs [step])
+    \\ gvs [with_atoms_def,force_list_def]
+    \\ rename [‘env_rel tenv senv’]
+    \\ drule_all_then (qspecl_then [‘SOME ss’,‘AppK senv AppOp [Constructor "" []] []::
+             AppK senv AppOp [Constructor "" []] []::sk’]
+         strip_assume_tac) eval_thm \\ gvs []
+    >-
+     (pop_assum $ qspec_then ‘k’ strip_assume_tac \\ gvs []
+      \\ qexists_tac ‘ck’ \\ fs [])
+    \\ gvs [AllCaseEqs()]
+    \\ Q.REFINE_EXISTS_TAC ‘ck1+ck’ \\ rewrite_tac [step_n_add] \\ fs [step]
+    \\ Cases_on ‘tv’ \\ fs [get_atoms_def]
+    \\ Cases_on ‘l’ \\ gvs [GSYM PULL_FORALL,PULL_EXISTS]
+    \\ pop_assum mp_tac
+    \\ simp [Once v_rel_cases]
+    \\ strip_tac \\ gvs []
+    \\ rpt (first_assum $ irule_at Any)
+    \\ qexists_tac ‘senv’
+    \\ Q.REFINE_EXISTS_TAC ‘ck1+1’ \\ rewrite_tac [step_n_add] \\ fs [step]
+    \\ Q.REFINE_EXISTS_TAC ‘ck1+1’ \\ rewrite_tac [step_n_add] \\ fs [step]
+    \\ Q.REFINE_EXISTS_TAC ‘ck1+1’ \\ rewrite_tac [step_n_add] \\ fs [step]
+    \\ Q.REFINE_EXISTS_TAC ‘ck1+1’ \\ rewrite_tac [step_n_add] \\ fs [step]
+    \\ qexists_tac ‘0’ \\ fs [])
+  \\ Cases_on ‘s = "Alloc"’ >-
+   (reverse (Cases_on ‘LENGTH vs = 2’) >- fs [Once next_def]
+    \\ once_rewrite_tac [next_def] \\ fs []
+    \\ cheat)
+  \\ Cases_on ‘s = "Length"’ >-
+   (reverse (Cases_on ‘LENGTH vs = 1’) >- fs [Once next_def]
+    \\ once_rewrite_tac [next_def] \\ fs []
+    \\ cheat)
+  \\ Cases_on ‘s = "Deref"’ >-
+   (reverse (Cases_on ‘LENGTH vs = 2’) >- fs [Once next_def]
+    \\ once_rewrite_tac [next_def] \\ fs []
+    \\ cheat)
+  \\ Cases_on ‘s = "Update"’ >-
+   (reverse (Cases_on ‘LENGTH vs = 3’) >- fs [Once next_def]
+    \\ once_rewrite_tac [next_def] \\ fs []
+    \\ cheat)
+  \\ once_rewrite_tac [next_def] \\ fs []
+QED
+
+Theorem next_eval_thm:
   ∀k e1 e2 tk sk senv tenv tres ts ss.
     compile_rel e1 e2 ∧
     LIST_REL (LIST_REL v_rel) ts ss ∧
@@ -645,10 +937,7 @@ Theorem next_thm:
            cont_rel tk sk ∧ sk1 = AppK nenv AppOp [Constructor "" []] []::sk ∧
            LIST_REL (LIST_REL v_rel) ts1 ss1)
 Proof
-
-  gen_tac \\ completeInduct_on ‘k’
-  \\ gvs [PULL_FORALL,AND_IMP_INTRO] \\ rw []
-  \\ pop_assum mp_tac
+  rw [] \\ pop_assum mp_tac
   \\ Cases_on ‘eval tenv e1 = INL Type_error’ \\ fs []
   >- simp [Once next_def]
   \\ Cases_on ‘eval tenv e1 = INL Diverge’ \\ fs []
@@ -678,56 +967,13 @@ Proof
   \\ rpt strip_tac
   \\ Q.REFINE_EXISTS_TAC ‘ck1+ck'’
   \\ rewrite_tac [step_n_add] \\ fs [step_def,push_def]
-  \\ ntac 2 $ pop_assum mp_tac
-  \\ Cases_on ‘s = "Ret"’ >-
-
-   (reverse (Cases_on ‘LENGTH vs = 1’) >- fs [Once next_def]
-    \\ once_rewrite_tac [next_def] \\ gvs []
-    \\ simp [Once v_rel_cases,monad_cns_def]
-    \\ strip_tac \\ gvs []
-    \\ Cases_on ‘tk’ \\ fs []
-    >-
-     (Q.REFINE_EXISTS_TAC ‘ck1+1’
-      \\ rewrite_tac [step_n_add]
-      \\ fs [step_def,push_def,return_def,value_def,opt_bind_def,continue_def,
-             application_def,dest_anyClosure_def,dest_Closure_def]
-      \\ qexists_tac ‘1’ \\ fs [step_def,value_def,GSYM PULL_FORALL]
-      \\ fs [cont_rel_cases,is_halt_def])
-    \\ cheat)
-
-  \\ Cases_on ‘s = "Raise"’ >-
-   (reverse (Cases_on ‘LENGTH vs = 1’) >- fs [Once next_def]
-    \\ once_rewrite_tac [next_def] \\ fs []
-    \\ cheat)
-  \\ Cases_on ‘s = "Bind"’ >-
-   (reverse (Cases_on ‘LENGTH vs = 2’) >- fs [Once next_def]
-    \\ once_rewrite_tac [next_def] \\ fs []
-    \\ cheat)
-  \\ Cases_on ‘s = "Handle"’ >-
-   (reverse (Cases_on ‘LENGTH vs = 2’) >- fs [Once next_def]
-    \\ once_rewrite_tac [next_def] \\ fs []
-    \\ cheat)
-  \\ Cases_on ‘s = "Act"’ >-
-   (reverse (Cases_on ‘LENGTH vs = 1’) >- fs [Once next_def]
-    \\ once_rewrite_tac [next_def] \\ fs []
-    \\ cheat)
-  \\ Cases_on ‘s = "Alloc"’ >-
-   (reverse (Cases_on ‘LENGTH vs = 2’) >- fs [Once next_def]
-    \\ once_rewrite_tac [next_def] \\ fs []
-    \\ cheat)
-  \\ Cases_on ‘s = "Length"’ >-
-   (reverse (Cases_on ‘LENGTH vs = 1’) >- fs [Once next_def]
-    \\ once_rewrite_tac [next_def] \\ fs []
-    \\ cheat)
-  \\ Cases_on ‘s = "Deref"’ >-
-   (reverse (Cases_on ‘LENGTH vs = 2’) >- fs [Once next_def]
-    \\ once_rewrite_tac [next_def] \\ fs []
-    \\ cheat)
-  \\ Cases_on ‘s = "Update"’ >-
-   (reverse (Cases_on ‘LENGTH vs = 3’) >- fs [Once next_def]
-    \\ once_rewrite_tac [next_def] \\ fs []
-    \\ cheat)
-  \\ once_rewrite_tac [next_def] \\ fs []
+  \\ ‘∃res. next k (INR (Constructor s vs)) tk ts = res’ by fs []
+  \\ fs []
+  \\ drule_all next_thm
+  \\ disch_then (qspec_then ‘senv’ strip_assume_tac)
+  \\ first_x_assum $ irule_at Any
+  \\ Cases_on ‘res’ \\ fs []
+  \\ PairCases_on ‘e’ \\ fs []
 QED
 
 Theorem next_action_thm:
@@ -756,7 +1002,7 @@ Proof
     \\ ‘∃s. next x (eval tenv e1) tk ts = s’ by fs []
     \\ ‘s = Div’ by metis_tac []
     \\ ‘s ≠ Err ∧ x ≤ x’ by gvs []
-    \\ drule_all next_thm \\ fs []
+    \\ drule_all next_eval_thm \\ fs []
     \\ strip_tac \\ gvs []
     \\ ‘x = n ∨ x < n’ by fs [] \\ gvs []
     \\ strip_tac
@@ -774,7 +1020,7 @@ Proof
   \\ rpt (disch_then strip_assume_tac)
   >-
    (CCONTR_TAC
-    \\ drule_all next_thm
+    \\ drule_all next_eval_thm
     \\ fs []
     >- metis_tac  []
     \\ PairCases_on ‘a’ \\ fs []
@@ -784,7 +1030,7 @@ Proof
   \\ ‘∃t. (step_n x'
              (Exp senv e2,SOME ss,AppK senv AppOp [Constructor "" []] []::sk)) = t’ by fs []
   \\ PairCases_on ‘t’ \\ fs []
-  \\ drule_all next_thm \\ fs []
+  \\ drule_all next_eval_thm \\ fs []
   \\ strip_tac
   \\ ‘(sres',ss0,sk1) = (t0,t1,t2)’ by
    (qpat_x_assum ‘is_halt (t0,t1,t2)’ mp_tac
@@ -909,7 +1155,7 @@ Proof
   fs [env_semanticsTheory.itree_of_def,
       stateLangTheory.itree_of_def] \\ rw []
   \\ irule semantics_thm
-  \\ simp [cont_rel_cases]
+  \\ simp [Once cont_rel_cases]
   \\ fs [env_rel_def]
 QED
 
